srv.v
@@ -1,0 +1,52 @@
+From iris.program_logic Require Export weakestpre.
+From iris.proofmode Require Import invariants ghost_ownership.
+From iris.heap_lang Require Export lang.
+From iris.heap_lang Require Import proofmode notation.
+From iris.heap_lang.lib Require Import spin_lock.
+From iris.algebra Require Import frac excl dec_agree.
+
+Definition srv : val :=
+  rec: "srv" "f" "p" :=
+       match: !"p" with
+         InjL "x" => "p" <- InjR ("f" "x");; "srv" "f" "p"
+       | InjR "_" => "srv" "f" "p"
+       end.
+
+Definition mk_srv : val :=
+  λ: "f",
+     let: "l" := newlock #() in
+     let: "p" := ref (InjR #0)%V in
+     Fork (srv "f" "p");;
+     rec: "wait" "x" :=
+        acquire "l";;
+        "p" <- InjL "x"
+        match: !"p" with
+          InjR "r" => "p" <- #0 ;; "r"
+        | InjL "_" => "wait" "x"
+        end.
+
+(* play with some algebraic structure to see what fit ... *)
+
+Definition srvR := prodR fracR (dec_agreeR val).
+
+Lemma srv_coincide: ∀ (x1 x2: val) (q1 q2: Qp), ✓ ((q1, DecAgree x1) ⋅ (q2, DecAgree x2)) → x1 = x2.
+Proof.
+  intros x1 x2 q1 q2 H. destruct (decide (x1 = x2))=>//.
+  exfalso. destruct H as [H1 H2].
+  simpl in H2. apply dec_agree_op_inv in H2.
+  by inversion H2.
+Qed.
+
+Lemma srv_update: ∀ (x1 x2: val), (1%Qp, DecAgree x1) ~~> (1%Qp, DecAgree x2).
+Proof. intros. by apply cmra_update_exclusive. Qed.
+
+(* define the gFunctors *)
+Class srvG Σ := FlatG { srv_tokG :> inG Σ srvR }.
+Definition srvΣ : gFunctors := #[GFunctor (constRF srvR)].
+
+Instance subG_srvΣ {Σ} : subG srvΣ Σ → srvG Σ.
+Proof. intros [?%subG_inG _]%subG_inv. split; apply _. Qed.
+
+Section proof.
+  Context `{!heapG Σ, !lockG Σ, !srvG Σ} (N : namespace).
+  
